### 3.10

$Z(t)= \sum_{k=1}^{n} X_ke^{j (\omega_0t+\Phi_k)}$

$m_z(t)$

$= E \{ Z_t\}$

$= E ( \sum_{k=1}^{n} X_ke^{j (\omega_0t+\Phi_k)})$

$= \sum_{k=1}^{n}E (  X_ke^{j (\omega_0t+\Phi_k)})$

$= \sum_{k=1}^{n} (E(X_k) E(e^{j \omega_0t+\Phi_k}))$

由题可知 $E(X_k) = 0$ , 故 $m_z(t)=0$ 。



$R_z(s,t)$

$=E \{ Z_s \overline{Z_t}\}$

$=E ( \sum_{k=1}^{n} X_ke^{j (\omega_0s+\Phi_k)} \overline{\sum_{k=1}^{n} X_ke^{j (\omega_0t+\Phi_k)}})$ 

$=E ( \sum_{k=1}^{n} X_ke^{j (\omega_0s+\Phi_k)} \sum_{k=1}^{n} X_ke^{-j (\omega_0t+\Phi_k)})$ 

$=E ( \sum_{k=1}^{n}\sum_{l=1}^{n} X_ke^{j (\omega_0s+\Phi_k)} X_le^{-j (\omega_0t+\Phi_l)})$  

$=\sum_{k=1}^{n}\sum_{l=1}^{n} E(X_ke^{j (\omega_0s+\Phi_k)} X_le^{-j (\omega_0t+\Phi_l)})$​  

$=\sum_{k=1}^{n}\sum_{l=1}^{n} E(X_kX_l)E(e^{j (\omega_0s+\Phi_k)} Xe^{-j (\omega_0t+\Phi_l)})$ 

已知 ${X_n}$ 相对独立，因此$\forall k,l$ if $k \ne l$ then $E(X_lX_k)=0$

故

$\sum_{k=1}^{n}\sum_{l=1}^{n} E(X_kX_l)E(e^{j (\omega_0s+\Phi_k)} Xe^{-j (\omega_0t+\Phi_l)})$

$= \sum_{k=1}^{n}E(X_k^2)e^{j \omega_0(s-t)}$

$= \sum_{k=1}^{n}D(X_k)e^{j \omega_0(s-t)}$

$= \sum_{k=1}^{n}\sigma_k^2 e^{j \omega_0(s-t)}$

$= \sum_{k=1}^{n}\sigma_k^2 e^{j \omega_0(s-t)}$

综上$R_z(s,t)=e^{j \omega_0(s-t)}\sum_{k=1}^{n}\sigma_k^2$



### 3.11

$R_Y(s,t) = E(Y_s, \overline{Y_t})$

$=E((X_s(t+a)-X_s(t)) \overline{(X_t(t+a)-X_t(t))})$

$=E((X_s(t+a)-X_s(t)) (\overline{X_t(t+a)}- \overline{X_t(t)}))$

$=E(X_{s+a} \overline{X_{t+a}}) - E(X_{s+a}\overline{X_t}) - E(X_s\overline{X_{t+a}}) + E(X_s\overline{X_t})$ 

$=R_X(s+a,t+a)-R_X(s+a,t)-R_X(s,t+a)+R_X(s,t)$
